Simplify QuickCheck implementation

base/coq/Free/Class/Handler.v
@@ -6,12 +6,12 @@ Class Handler (Shape : Type) (Pos : Shape -> Type) (A : Type) := {
   (* This function defines how a type is transformed by the handling process.
      Does not usually have to be implemented when defining an instance, as
      it can be inferred from the type of handle. *)
-  handledType : Type;
+  handledType : Normalform Shape Pos A -> Type;
   (* This function defines how the given effect stack is handled.
      Its return type is the return type of the normalization as
      transformed by the handler.
      For example, for a handler for the effect stack containing only the Maybe
      effect, a Free Shape Pos (Bool Shape Pos) is turned into an
      option (Bool Identity.Shape Identity.Pos). *)
-  handle : Free Shape Pos A -> handledType
+  handle : forall {NF : Normalform Shape Pos A}, Free Shape Pos A -> handledType NF
 }.
