base/coq/Test/QuickCheck.v
@@ -4,11 +4,13 @@ From Base Require Import Prelude.
 From Base Require Import Free.Instance.Comb.
 From Base Require Import Free.Instance.Maybe.
 
-(* QuickCheck properties are implemented as Coq propositions. *)
-Definition Property (Shape : Type) (Pos : Shape -> Type) := forall (handler : forall (A : Type) (NF : Normalform Shape Pos A),
- Handler Shape Pos A), Prop.
+(* QuickCheck properties are implemented as Coq propositions
+   that are parameterized over a handler. The handler is used
+   when comparing values with [(===)] and [(=/=)]. *)
+Definition Property (Shape : Type) (Pos : Shape -> Type) : Type
+ := (forall (A : Type), Handler Shape Pos A) -> Prop.
 
-(* ShareableArgs instance for Property. *)
+(* [ShareableArgs] instance for [Property]. *)
 Instance ShareableArgsProperty (Shape : Type) (Pos : Shape -> Type)
   : ShareableArgs Shape Pos (Property Shape Pos) := {
     shareArgs _ := pure
@@ -17,127 +19,95 @@ Instance ShareableArgsProperty (Shape : Type) (Pos : Shape -> Type)
 (* * [Testable] type class *)
 
 (* [class Testable prop where property :: prop -> Property] *)
-Class Testable (prop : Type) := {
-  property' : prop -> Prop;
-  property : prop -> Prop
+Class Testable (Shape : Type) (Pos : Shape -> Type) (prop : Type) := {
+  property : prop -> Property Shape Pos
 }.
-
-(* [instance Testable Prop] *)
-Instance TestableProp
-  : Testable Prop
- := { property' p := p;
-      property p := p }.
 
 (* [instance Testable Property] *)
 Instance TestableProperty (Shape : Type) (Pos : Shape -> Type)
-  : Testable (Property Shape Pos)
- := { property' p := forall (handler : forall (A : Type) (NF : Normalform Shape Pos A),
-                             Handler Shape Pos A), p handler;
-      property p := p (NoHandler Shape Pos) }.
+  : Testable Shape Pos (Property Shape Pos)
+ := { property p := p }.
 
 (* [instance Testable Bool] *)
-Instance TestableBool
-  : Testable bool
- := { property' b := b = true;
-      property b := b = true }.
+Instance TestableBool (Shape : Type) (Pos : Shape -> Type)
+  : Testable Shape Pos (Bool Shape Pos)
+ := { property b _ := b = true }.
 
 (* [instance Testable b => Testable (a -> b)] *)
-Instance TestableFunction (A : Type) (B : Type) (T_B : Testable B)
-  : Testable (A -> B)
- := { property' f := forall x, property' (f x);
-      property f := forall x, property (f x) }.
+Instance TestableFunction
+  (Shape : Type) (Pos : Shape -> Type)
+  (A : Type) (B : Type) (T_B : Testable Shape Pos B)
+  : Testable Shape Pos (A -> B)
+ := { property f handler := forall x, property (f x) handler }.
 
 (* Helper instance for dependent types.
    This allows us to use [quickCheck] both for proving properties for specific
    and for arbitrary effects by providing a default strategy for how the
    binders for [Shape] and [Pos] can be converted to properties. *)
 Instance TestableForall
-  (A : Type) (B : A -> Type) (T_Bx : forall x, Testable (B x))
-  : Testable (forall x, B x)
- := { property' f := forall x, property' (f x);
-      property f := forall x, property (f x); }.
+  (Shape : Type) (Pos : Shape -> Type)
+  (A : Type) (B : A -> Type) (T_Bx : forall x, Testable Shape Pos (B x))
+  : Testable Shape Pos (forall x, B x)
+ := { property f handler := forall x, property (f x) handler }.
 
-(* Helper instance for monadically lifted values.
-
-   This instance defines the strategy for how to handle the computation of
-   a Coq property by a QuickCheck property defined in Haskell.
-   Here we say that a property must produce a [pure] value, otherwise it does
-   not hold. In case of the effect of partiality, this means that the
-   QuickCheck property [prop_undefined = undefined] is not satisfied.
-   (Note that due to the non-strict definition of [(===)] the property
-   [prop_undefined_eq = undefined === undefined] would still be true)
-
-   Whether this strategy makes sense in case of other effects such as
-   non-determinism still has to be investigated. For example, does the
-   property [prop_true_or_false = True ? False] hold or not? With the
-   current implementation it does not hold since the choice operator
-   produces an [impure] value.
-   *)
+(* Helper instance for monadically lifted values. *)
 Instance TestableFree (Shape : Type) (Pos : Shape -> Type)
-                      (A : Type) (T_A : Testable A)
-  : Testable (Free Shape Pos A)
- := { property' fp := match fp with
-                      | pure p     => property' p
-                      | impure _ _ => False
-                      end;
-      property fp := match fp with
-                      | pure p     => property p
-                      | impure _ _ => False
-                      end }.
-
-(* Similar to Testable, but returns a Property instead of a Prop so
-   that a handler can be applied. *)
-Class Handleable (Shape : Type) (Pos : Shape -> Type) (prop : Type) :=
-  {  toProperty : prop -> Property Shape Pos }.
-
-Instance HandleableBool (Shape : Type) (Pos : Shape -> Type)
-  : Handleable Shape Pos (Bool Shape Pos)
- := { toProperty b := fun _ => b = true }.
-
-Instance HandleableProperty (Shape : Type) (Pos : Shape -> Type) : Handleable Shape Pos (Property Shape Pos) := {
-  toProperty p := p
-}.
-
-Instance HandleableFree (Shape : Type) (Pos : Shape -> Type) {A : Type} {H_A : Handleable Shape Pos A} : Handleable Shape Pos (Free Shape Pos A) := {
-  toProperty fp := match fp with
-                   | pure p => toProperty p
-                   | impure s pf => (fun _ => False)
-                   end }.
-
-Instance HandleableFunction (Shape : Type) (Pos : Shape -> Type) (A : Type) (B : Type)
- (T_B : Handleable Shape Pos B)
-  : Handleable Shape Pos (A -> B)
- := { toProperty f := fun handler => forall x, toProperty (f x) handler }.
-
-Instance HandleableForall (Shape : Type) (Pos : Shape -> Type)
-  (A : Type) (B : A -> Type) (T_Bx : forall x, Handleable Shape Pos (B x))
-  : Handleable Shape Pos (forall x, B x)
- := { toProperty f := fun handler => forall x, toProperty (f x) handler }.
-
+                      (A : Type) (T_A : Testable Shape Pos A)
+  : Testable Shape Pos (Free Shape Pos A)
+ := { property fp handler := match fp with
+                             | pure p => property p handler
+                             | impure s pf => False
+                             end }.
 
 (* [quickCheck :: Testable a => a -> IO ()]
-   In Haskell this function is used to test a QuickCheck property.
-   We are reusing the name to convert the computation of a quickCheck
-   property to a Coq property that can actually be proven. *)
-Definition quickCheck {A : Type} {T_A : Testable A} (x : A) : Prop
- := property x.
 
-(* Like [quickCheck], but with a concrete handler as an additional argument.
+   In Haskell this function is used to test a QuickCheck property.
+   We are reusing the name to convert the computation of a QuickCheck
+   property to a Coq property that can actually be proven. *)
+Definition quickCheck
+  {A    : forall Shape Pos, Type}
+  {T_A  : forall Shape Pos, Testable Shape Pos (A Shape Pos)}
+  (prop : forall Shape Pos, A Shape Pos)
+  : Prop
+ := forall Shape Pos, property (prop Shape Pos) (NoHandler Shape Pos).
+
+(* Like [quickCheck] but with additional arguments for the [Shape] and
+   [Pos]ition.
+
+   You should use this function than [Shape] and [Pos] have been introduced
+   by an explicit [forall] already, e.g., because there are preconditions
+   that cannot be formulated in Haskell. *)
+Definition quickCheck'
+   {Shape : Type} {Pos : Shape -> Type}
+   {A : Type} {T_A : Testable Shape Pos A}
+   (prop : A)
+   : Prop
+ := property prop (NoHandler Shape Pos).
+
+(* Like [quickCheck] but with a concrete handler as an additional argument.
    The property's [Shape] and [Pos] arguments must be inferred or match
    the effect stack determined by the handler. *)
-Definition quickCheckHandle {Shape : Type} {Pos : Shape -> Type} {A : Type} `{Handleable Shape Pos A}
- (x : A) handler : Prop := (toProperty x) handler.
+Definition quickCheckHandle
+  {Shape} {Pos : Shape -> Type}
+  {A : Type} {T_A : Testable Shape Pos A}
+  (prop : A)
+  (handler : forall (A : Type), Handler Shape Pos A)
+  : Prop
+ := property prop handler.
 
-(* Like [quickCheck], but with a universally quantified handler.
-   Proving an equality with a universally quantified handler is
-   equivalent to proving the same equality without the handler.
-   Proving an inequality is impossible as there is no information
-   about the return value or even return type of the handler.
+(* Utility function to specify the evaluation strategy of a property without
+   having to bind the [Shape] and [Pos] explicitly.
 
-   As long as there are no properties associated with the handler
-   class, it is not advised to use this function. *)
-Definition quickCheckQuantifyHandler {A : Type} {T_A : Testable A} (x : A) : Prop
- := property' x.
+   This function is used as follows:
+   [quickCheck (withStrategy Cbn prop_foo)].
+ *)
+Definition withStrategy
+  {A    : forall Shape Pos, Type}
+  (S    : forall Shape Pos, Strategy Shape Pos)
+  (prop : forall Shape Pos (S : Strategy Shape Pos), A Shape Pos)
+  (Shape : Type) (Pos : Shape -> Type)
+  : A Shape Pos
+ := prop Shape Pos (S Shape Pos).
 
 (* * Constructing QuickCheck Properties *)
 Section SecQuickCheck.
@@ -152,22 +122,25 @@ Section SecQuickCheck.
      class instance for [Bool] is accessable from Haskell. *)
   Definition boolProp (fb : Free' Bool')
     : Free' Property'
-   := pure (fun handler => toProperty fb handler).
+   := pure (fun handler => property fb handler).
 
   (* [(==>) :: Bool -> Property -> Property] *)
-  Definition preProp (fb : Free' Bool') (p : Free' Property')
+  Definition preProp (fb : Free' Bool') (fp : Free' Property')
     : Free' Property'
-   := pure (fun handler => toProperty fb handler -> toProperty p handler).
+   := pure (fun handler => property fb handler -> property fp handler).
+
+  (* Version of [preProp] that allows arbitrary preconditions. *)
+  Definition preProp' (fx : Free' Property') (fy : Free' Property')
+    : Free' Property'
+   := pure (fun handler => property fx handler -> property fy handler).
 
   (* [(===) :: a -> a -> Property] *)
-  Definition eqProp (A : Type) `(NF : Normalform Shape Pos A)
-    (fx : Free' A) (fy : Free' A)
+  Definition eqProp (A : Type) `{Normalform Shape Pos A} (fx : Free' A) (fy : Free' A)
     : Free' Property'
    := pure (fun handler => handle fx = handle fy).
 
   (* [(=/=) :: a -> a -> Property] *)
-  Definition neqProp (A : Type) `(NF : Normalform Shape Pos A)
-                     (fx : Free' A) (fy : Free' A)
+  Definition neqProp (A : Type) `{Normalform Shape Pos A} (fx : Free' A) (fy : Free' A)
     : Free' Property'
    := pure (fun handler => handle fx <> handle fy).
 
@@ -190,23 +163,9 @@ End SecQuickCheck.
 Lemma pure_bool_property:
   forall (Shape : Type)
          (Pos : Shape -> Type)
-         (fb : Free Shape Pos (Bool Shape Pos)),
-  property fb <-> fb = True_ Shape Pos.
-Proof.
-  simpl. intros Shape Pos fb. split; intros H.
-  - (* -> *) destruct fb as [b |].
-    + (* fb = pure b *) rewrite H. reflexivity.
-    + (* fb = impure _ _ *) contradiction H.
-  - (* <- *) rewrite H. reflexivity.
-Qed.
-
-(* Helper lemma to avoid the [match] expression introduced by [toProperty]. *)
-Lemma pure_bool_toProperty:
-  forall (Shape : Type)
-         (Pos : Shape -> Type)
          (fb : Free Shape Pos (Bool Shape Pos))
-         handler,
-  toProperty fb handler <-> fb = True_ Shape Pos.
+         (handler : forall (A : Type), Handler Shape Pos A),
+  property fb handler <-> fb = True_ Shape Pos.
 Proof.
   simpl. intros Shape Pos fb. split; intros H.
   - (* -> *) destruct fb as [b |].
