base/coq/Free/Strategy/CallByName.v
@@ -4,3 +4,7 @@ Definition callByName (Shape : Type) (Pos : Shape -> Type)
   {A : Type} (p : Free Shape Pos A)
   : Free Shape Pos (Free Shape Pos A) :=
   pure p.
+
+(* When simplifying expressions, we want Coq to expand applications of
+   [callByName] such that the code becomes more readable. *)
+Arguments callByName Shape Pos {A} p /.
