base/coq/Free/Strategy/CallByValue.v
@@ -4,3 +4,7 @@ Definition callByValue (Shape : Type) (Pos : Shape -> Type)
   {A : Type} (p : Free Shape Pos A)
   : Free Shape Pos (Free Shape Pos A) :=
   p >>= fun x => pure (pure x).
+
+(* When simplifying expressions, we want Coq to expand applications of
+   [callByValue] such that the code becomes more readable. *)
+Arguments callByValue Shape Pos {A} p /.
