example/Base/StrategyProofs.v
@@ -3,114 +3,114 @@ From Generated Require Import Base.Strategy.
 
 (* Proofs for Tracing Test Functions *)
 
-Example add_traced_cbv : quickCheckHandle (@prop_add_traced_cbv _ _ Cbv _) HandlerTrace.
+Example add_traced_cbv : quickCheckHandle (@prop_add_traced_cbv _ _ cbv _) HandlerTrace.
 Proof. constructor. Qed.
 
-Example add_traced_cbn : quickCheckHandle (@prop_add_traced_cbn _ _ Cbn _) HandlerTrace.
+Example add_traced_cbn : quickCheckHandle (@prop_add_traced_cbn _ _ cbn _) HandlerTrace.
 Proof. constructor. Qed.
 
-Example add_traced_cbneed : quickCheckHandle (@prop_add_traced_cbneed _ _ Cbneed _) HandlerShareTrace.
-Proof. constructor. Qed.
-
-
-Example or_true_traced_cbv : quickCheckHandle (@prop_or_true_traced_cbv _ _ Cbv _) HandlerTrace.
-Proof. constructor. Qed.
-
-Example or_true_traced_cbn : quickCheckHandle (@prop_or_true_traced_cbn _ _ Cbn _) HandlerTrace.
-Proof. constructor. Qed.
-
-Example or_true_traced_cbneed : quickCheckHandle (@prop_or_true_traced_cbneed _ _ Cbneed _) HandlerShareTrace.
+Example add_traced_cbneed : quickCheckHandle (@prop_add_traced_cbneed _ _ cbneed _) HandlerShareTrace.
 Proof. constructor. Qed.
 
 
-Example or_false_traced_cbv : quickCheckHandle (@prop_or_false_traced_cbv _ _ Cbv _) HandlerTrace.
+Example or_true_traced_cbv : quickCheckHandle (@prop_or_true_traced_cbv _ _ cbv _) HandlerTrace.
 Proof. constructor. Qed.
 
-Example or_false_traced_cbn : quickCheckHandle (@prop_or_false_traced_cbn _ _ Cbn _) HandlerTrace.
+Example or_true_traced_cbn : quickCheckHandle (@prop_or_true_traced_cbn _ _ cbn _) HandlerTrace.
 Proof. constructor. Qed.
 
-Example or_false_traced_cbneed : quickCheckHandle (@prop_or_false_traced_cbneed _ _ Cbneed _) HandlerShareTrace.
-Proof. constructor. Qed.
-
-
-Example true_or_false_traced_cbv : quickCheckHandle (@prop_true_or_false_traced_cbv _ _ Cbv _) HandlerTrace.
-Proof. constructor. Qed.
-
-Example true_or_false_traced_cbn : quickCheckHandle (@prop_true_or_false_traced_cbn _ _ Cbn _) HandlerTrace.
-Proof. constructor. Qed.
-
-Example true_or_false_traced_cbneed : quickCheckHandle (@prop_true_or_false_traced_cbneed _ _ Cbneed _) HandlerShareTrace.
+Example or_true_traced_cbneed : quickCheckHandle (@prop_or_true_traced_cbneed _ _ cbneed _) HandlerShareTrace.
 Proof. constructor. Qed.
 
 
-Example false_or_true_traced_cbv : quickCheckHandle (@prop_false_or_true_traced_cbv _ _ Cbv _) HandlerTrace.
+Example or_false_traced_cbv : quickCheckHandle (@prop_or_false_traced_cbv _ _ cbv _) HandlerTrace.
 Proof. constructor. Qed.
 
-Example false_or_true_traced_cbn : quickCheckHandle (@prop_false_or_true_traced_cbn _ _ Cbn _) HandlerTrace.
+Example or_false_traced_cbn : quickCheckHandle (@prop_or_false_traced_cbn _ _ cbn _) HandlerTrace.
 Proof. constructor. Qed.
 
-Example false_or_true_traced_cbneed : quickCheckHandle (@prop_false_or_true_traced_cbneed _ _ Cbneed _) HandlerShareTrace.
+Example or_false_traced_cbneed : quickCheckHandle (@prop_or_false_traced_cbneed _ _ cbneed _) HandlerShareTrace.
 Proof. constructor. Qed.
 
 
-Example partial_traced_cbv : quickCheckHandle (@prop_partial_traced_cbv _ _ Cbv _ _) HandlerMaybeTrace.
+Example true_or_false_traced_cbv : quickCheckHandle (@prop_true_or_false_traced_cbv _ _ cbv _) HandlerTrace.
 Proof. constructor. Qed.
 
-Example partial_traced_cbn : quickCheckHandle (@prop_partial_traced_cbn _ _ Cbn _ _) HandlerMaybeTrace.
+Example true_or_false_traced_cbn : quickCheckHandle (@prop_true_or_false_traced_cbn _ _ cbn _) HandlerTrace.
 Proof. constructor. Qed.
 
-Example partial_traced_cbneed : quickCheckHandle (@prop_partial_traced_cbneed _ _ Cbneed _ _) HandlerMaybeShareTrace.
+Example true_or_false_traced_cbneed : quickCheckHandle (@prop_true_or_false_traced_cbneed _ _ cbneed _) HandlerShareTrace.
+Proof. constructor. Qed.
+
+
+Example false_or_true_traced_cbv : quickCheckHandle (@prop_false_or_true_traced_cbv _ _ cbv _) HandlerTrace.
+Proof. constructor. Qed.
+
+Example false_or_true_traced_cbn : quickCheckHandle (@prop_false_or_true_traced_cbn _ _ cbn _) HandlerTrace.
+Proof. constructor. Qed.
+
+Example false_or_true_traced_cbneed : quickCheckHandle (@prop_false_or_true_traced_cbneed _ _ cbneed _) HandlerShareTrace.
+Proof. constructor. Qed.
+
+
+Example partial_traced_cbv : quickCheckHandle (@prop_partial_traced_cbv _ _ cbv _ _) HandlerMaybeTrace.
+Proof. constructor. Qed.
+
+Example partial_traced_cbn : quickCheckHandle (@prop_partial_traced_cbn _ _ cbn _ _) HandlerMaybeTrace.
+Proof. constructor. Qed.
+
+Example partial_traced_cbneed : quickCheckHandle (@prop_partial_traced_cbneed _ _ cbneed _ _) HandlerMaybeShareTrace.
 Proof. constructor. Qed.
 
 
 (* Proofs for Non-Determinism Test Functions *)
 
-Example add_non_det_cbv : quickCheckHandle (@prop_add_non_det_cbv _ _ Cbv _) HandlerND.
+Example add_non_det_cbv : quickCheckHandle (@prop_add_non_det_cbv _ _ cbv _) HandlerND.
 Proof. constructor. Qed.
 
-Example add_non_det_cbn : quickCheckHandle (@prop_add_non_det_cbn _ _ Cbn _) HandlerND.
+Example add_non_det_cbn : quickCheckHandle (@prop_add_non_det_cbn _ _ cbn _) HandlerND.
 Proof. constructor. Qed.
 
-Example add_non_det_cbneed : quickCheckHandle (@prop_add_non_det_cbneed _ _ Cbneed _) HandlerShareND.
-Proof. constructor. Qed.
-
-
-Example or_true_false_non_det_cbv : quickCheckHandle (@prop_or_true_false_non_det_cbv _ _ Cbv _) HandlerND.
-Proof. constructor. Qed.
-
-Example or_true_false_non_det_cbn : quickCheckHandle (@prop_or_true_false_non_det_cbn _ _ Cbn _) HandlerND.
-Proof. constructor. Qed.
-
-Example or_true_false_non_det_cbneed : quickCheckHandle (@prop_or_true_false_non_det_cbneed _ _ Cbneed _) HandlerShareND.
+Example add_non_det_cbneed : quickCheckHandle (@prop_add_non_det_cbneed _ _ cbneed _) HandlerShareND.
 Proof. constructor. Qed.
 
 
-Example partial_non_det_cbv : quickCheckHandle (@prop_partial_non_det_cbv _ _ Cbv (Maybe.Partial _ _) _) HandlerNDMaybe.
+Example or_true_false_non_det_cbv : quickCheckHandle (@prop_or_true_false_non_det_cbv _ _ cbv _) HandlerND.
 Proof. constructor. Qed.
 
-Example partial_non_det_cbn : quickCheckHandle (@prop_partial_non_det_cbn _ _ Cbn (Maybe.Partial _ _) _) HandlerNDMaybe.
+Example or_true_false_non_det_cbn : quickCheckHandle (@prop_or_true_false_non_det_cbn _ _ cbn _) HandlerND.
 Proof. constructor. Qed.
 
-Example partial_non_det_cbneed : quickCheckHandle (@prop_partial_non_det_cbneed _ _ Cbneed (Maybe.Partial _ _) _) HandlerShareNDMaybe.
+Example or_true_false_non_det_cbneed : quickCheckHandle (@prop_or_true_false_non_det_cbneed _ _ cbneed _) HandlerShareND.
+Proof. constructor. Qed.
+
+
+Example partial_non_det_cbv : quickCheckHandle (@prop_partial_non_det_cbv _ _ cbv (Maybe.Partial _ _) _) HandlerNDMaybe.
+Proof. constructor. Qed.
+
+Example partial_non_det_cbn : quickCheckHandle (@prop_partial_non_det_cbn _ _ cbn (Maybe.Partial _ _) _) HandlerNDMaybe.
+Proof. constructor. Qed.
+
+Example partial_non_det_cbneed : quickCheckHandle (@prop_partial_non_det_cbneed _ _ cbneed (Maybe.Partial _ _) _) HandlerShareNDMaybe.
 Proof. constructor. Qed.
 
 (* Proofs for Deep Sharing Test Functions *)
 
-Example double_cbv : quickCheckHandle (@prop_double_cbv _ _ Cbv _) HandlerTrace.
+Example double_cbv : quickCheckHandle (@prop_double_cbv _ _ cbv _) HandlerTrace.
 Proof. constructor. Qed.
 
-Example double_cbn : quickCheckHandle (@prop_double_cbn _ _ Cbn _) HandlerTrace.
+Example double_cbn : quickCheckHandle (@prop_double_cbn _ _ cbn _) HandlerTrace.
 Proof. constructor. Qed.
 
-Example double_cbneed : quickCheckHandle (@prop_double_cbneed _ _ Cbneed _) HandlerShareTrace.
+Example double_cbneed : quickCheckHandle (@prop_double_cbneed _ _ cbneed _) HandlerShareTrace.
 Proof. constructor. Qed.
 
 
-Example double_maybe_cbv : quickCheckHandle (@prop_double_maybe_cbv _ _ Cbv _) HandlerTrace.
+Example double_maybe_cbv : quickCheckHandle (@prop_double_maybe_cbv _ _ cbv _) HandlerTrace.
 Proof. constructor. Qed.
 
-Example double_maybe_cbn : quickCheckHandle (@prop_double_maybe_cbn _ _ Cbn _) HandlerTrace.
+Example double_maybe_cbn : quickCheckHandle (@prop_double_maybe_cbn _ _ cbn _) HandlerTrace.
 Proof. constructor. Qed.
 
-Example double_maybe_cbneed : quickCheckHandle (@prop_double_maybe_cbneed _ _ Cbneed _) HandlerShareTrace.
+Example double_maybe_cbneed : quickCheckHandle (@prop_double_maybe_cbneed _ _ cbneed _) HandlerShareTrace.
 Proof. constructor. Qed.
