example/CaseStudyHuttonsRazor/RazorProofsMaybe.v
@@ -17,7 +17,7 @@ Section Proofs_Maybe.
   (* In the following proofs we use the [Maybe] monad in a call-by-name setting. *)
   Definition Shape   := Maybe.Shape.
   Definition Pos     := Maybe.Pos.
-  Definition S       := @Cbn Shape Pos.
+  Definition S       := Cbn Shape Pos.
   Definition Partial := Maybe.Partial Shape Pos.
 
   (* In the [Maybe] monad there exists only one impure value. *)
@@ -36,7 +36,7 @@ Section Proofs_Maybe.
   (* If the stack is impure the result of any [exec] call on that stack will be impure. *)
   Lemma exec_strict_on_stack_arg :
     forall (fcode  : Free Shape Pos (Code Shape Pos)),
-      exec Shape Pos Cbn Partial fcode (Nothing _ _) = Nothing _ _.
+      exec Shape Pos cbn Partial fcode (Nothing _ _) = Nothing _ _.
   Proof.
     intro fcode.
     destruct fcode as [ [ | [ [ fn | ] | sOp pfOp ] fcode1 ] | sCode pfCode ];
@@ -51,8 +51,8 @@ Section Proofs_Maybe.
     forall (fcode1 : Free Shape Pos (Code Shape Pos)),
     forall (fcode2 : Free Shape Pos (Code Shape Pos)),
     forall (fstack        : Free Shape Pos (Stack Shape Pos)),
-        exec Shape Pos Cbn Partial (append Shape Pos Cbn fcode1 fcode2) fstack
-        = exec Shape Pos Cbn Partial fcode2 (exec Shape Pos Cbn Partial fcode1 fstack).
+        exec Shape Pos cbn Partial (append Shape Pos cbn fcode1 fcode2) fstack
+        = exec Shape Pos cbn Partial fcode2 (exec Shape Pos cbn Partial fcode1 fstack).
   Proof.
     intros fcode1 fcode2.
     (* Destruct the monadic layer of the first piece of code. *)
@@ -114,8 +114,8 @@ Section Proofs_Maybe.
     RecPureExpr fexpr ->
     forall (fstack : Free Shape Pos (Stack Shape Pos)),
     RecPureStack fstack ->
-        exec Shape Pos Cbn Partial (comp Shape Pos Cbn fexpr) fstack
-        = Cons Shape Pos (eval Shape Pos Cbn fexpr) fstack.
+        exec Shape Pos cbn Partial (comp Shape Pos cbn fexpr) fstack
+        = Cons Shape Pos (eval Shape Pos cbn fexpr) fstack.
   Proof.
     intros N fexpr HPureE.
     destruct fexpr as [ expr | ]. 2: dependent destruction HPureE.
@@ -149,7 +149,7 @@ Section Proofs_Maybe.
   Lemma comp_correct :
     forall (fexpr : Free Shape Pos (Expr Shape Pos)),
     RecPureExpr fexpr ->
-        quickCheck (prop_comp_correct Shape Pos Cbn Partial fexpr).
+        quickCheck' (prop_comp_correct Shape Pos cbn Partial fexpr).
   Proof.
     intros fexpr HPureE.
     apply (comp_correct' fexpr HPureE (Nil Shape Pos) recPureStack_nil).
