example/Proofs/TracingProofs.v
@@ -1,7 +1,7 @@
 From Base Require Import Free Free.Handlers Prelude Test.QuickCheck.
 From Generated Require Import Proofs.Tracing.
 
-Theorem trace_is_shared : quickCheckHandle (@prop_trace_is_shared _ _ Cbneed _) HandlerShareTrace.
+Theorem trace_is_shared : quickCheckHandle (@prop_trace_is_shared _ _ cbneed _) HandlerShareTrace.
 Proof.
   simpl. reflexivity.
 Qed.
